Finish ring theory test, more tactics and improvements
tactic to start, simpler unfold_ctx tactic
Multi argument specialize
rewrite (H x) and similar tactics
Tactics are slow but ok for now
Delete old tests

test/TheoryTest.v
@@ -3,7 +3,7 @@
 Require Import Task.
 Require Import Theory.
 Require Import Typechecker.
-Require Import NatDed.
+Require Import Tactics.
 From mathcomp Require Import all_ssreflect.
 Set Bullet Behavior "Strict Subproofs".
 
@@ -468,585 +468,115 @@ Proof. check_theory. Qed.
 
 Require Import Alpha.
 
-Ltac prove_fmla_ty :=
-  apply /typecheck_formula_correct; reflexivity.
-
-Ltac prove_tm_ty :=
-  apply /check_tm_ty_spec; reflexivity.
-
-Definition check_formulas_typed (gamma: context) (l: list formula): bool :=
-  all (typecheck_formula gamma) l.
-
-Lemma check_formulas_typed_correct gamma l:
-  reflect (Forall (formula_typed gamma) l) (check_formulas_typed gamma l).
-Proof.
-  unfold check_formulas_typed.
-  apply forallb_ForallP. intros.
-  apply typecheck_formula_correct.
-Qed.
-
-Ltac prove_fmlas_ty :=
-  apply /check_formulas_typed_correct; reflexivity.
-
-Ltac prove_valid_context :=
-  apply /check_context_correct; reflexivity.
 
 (*Now, we prove these lemmas (manually, from the semantics)
   *)
 Notation "0r" :=(Tfun Ring.zero nil nil).
 Notation "x '+r' y" := (Tfun Ring.plus nil [x; y])
   (at level 60).
-Notation "'-r' x" := (Tfun Ring.neg nil x)
+Notation "'-r' x" := (Tfun Ring.neg nil [x])
   (at level 70).
 Notation "x '*r' y" := (Tfun Ring.mult nil [x;y])
   (at level 50).
 Notation "x '==' y" := (Feq _ x y).
 (*A complete hack*)
-Notation xt := (t_constsym ("x"%string) t_ty).
+Definition xt := (t_constsym ("x"%string) t_ty).
+Definition yt := (t_constsym ("y"%string) t_ty).
+Definition zt := (t_constsym ("z"%string) t_ty).
+
+Lemma xt_eq: Tfun (constsym "x" t_ty) nil nil = xt.
+Proof. reflexivity. Qed.
+Lemma yt_eq: Tfun (constsym "y" t_ty) nil nil = yt.
+Proof. reflexivity. Qed.
+Lemma zt_eq: Tfun (constsym "z" t_ty) nil nil = zt.
+Proof. reflexivity. Qed.
+
+
+Local Open Scope string_scope.
+
+(*Here, our extra_simpl task folds up our defined constants*)
+Ltac extra_simpl ::=
+  fold t_ty; fold x; fold y; fold z;
+  fold xt; fold yt; fold zt;
+  try rewrite !xt_eq;
+  try rewrite !yt_eq;
+  try rewrite !zt_eq.
+
 (*TODO: get some real notations*)
 Lemma ring_theory_valid: valid_theory ring_theory.
 Proof.
   simpl. split_all; auto.
   - (*First lemma*)
-    apply soundness.
-    simpl_task.
-    rewrite theory_axioms_ext_equation_1.
-    rewrite !app_nil_r.
+    wstart.  
     (*1.intros*)
-    apply D_forallI with(c:="x"%string).
-    reflexivity.
-    (*TODO: automate these*)
-    prove_fmlas_ty.
-    prove_closed.
-    (*TODO: safe_sub_f does not evaluate*)
-    unfold safe_sub_f; simpl.
+    wintros "x".
     (*So now we have to prove for a specific x, that x * 0 = 0 *)
     (*2. assert (0 + 0 = 0)*)
-    apply (D_assert _ _ (Feq t_ty (0r +r 0r) 0r)).
+    wassert "Hz" (Feq t_ty (0r +r 0r) 0r).
     {
-      (*Prove the assertion*)
-      (*We need a better way to do this*)
-      apply (D_assert _ _ (Fquant Tforall x 
-        (Feq t_ty (0r +r (Tvar x)) (Tvar x)))).
-      {
-        apply D_axiom.
-        prove_task_wf.
-        apply /inP. reflexivity.
-      }
-      (*Now we specialize*)
-      (*TODO: this is awful*)
-      apply (D_assert _ _ (safe_sub_f 0r x (Feq t_ty 
-        (0r +r Tvar x) (Tvar x)))).
-      {
-        apply D_forallE. prove_tm_ty.
-        (*TODO: decidable closed term*)
-        constructor; reflexivity.
-        apply D_axiom; [prove_task_wf | apply /inP; reflexivity].
-      }
-      unfold safe_sub_f; simpl. 
-      apply D_axiom; [prove_task_wf | apply /inP; reflexivity].
+      wrewrite["Unit_def_l" 0r].
+      wreflexivity.
+      (*Alternative (and faster)*)
+      (*
+      wspecialize "Unit_def_l" 0r.
+      wassumption.*)
     }
     (*3. From this and f_equal, we can prove that x * (0 + 0) = x * 0*)
-    apply (D_assert _ _ (Feq t_ty (xt *r (0r +r 0r)) (xt *r 0r))).
+    wassert "Hz2" (Feq t_ty (xt *r (0r +r 0r)) (xt *r 0r)).
     {
-      apply D_f_equal; try reflexivity; try prove_tm_ty.
-      simpl. (*Need better way to do this*) constructor.
-      - apply D_eq_refl; auto.
-        prove_valid_context.
-        prove_fmlas_ty.
-        constructor; reflexivity.
-        prove_tm_ty.
-      - constructor; [|constructor].
-        apply D_axiom; [prove_task_wf | apply /inP; reflexivity].
+      wf_equal.
+      - wreflexivity.
+      - wassumption.
     }
     (*4. we have that x * (0 + 0) = 0 + x * 0*)
-    apply (D_assert _ _ (Feq t_ty (xt *r (0r +r 0r)) (0r +r (xt *r 0r)))).
+    wassert "Hz3" (Feq t_ty (xt *r (0r +r 0r)) ((xt *r 0r) +r 0r)).
     {
-      apply D_rewrite with(t1:=0r +r (xt *r 0r))(t2:=xt *r 0r)(ty:=t_ty).
-      prove_closed.
-      - apply (D_assert _ _ (Fquant Tforall x 
-          (Feq t_ty (0r +r (Tvar x)) (Tvar x)))).
-        {
-          apply D_axiom.
-          prove_task_wf.
-          apply /inP. reflexivity.
-        }
-        (*Now we specialize*)
-        apply (D_assert _ _ (safe_sub_f (xt *r 0r) x (Feq t_ty 
-          (0r +r Tvar x) (Tvar x)))).
-        {
-          apply D_forallE. prove_tm_ty.
-          (*TODO: decidable closed term*)
-          constructor; reflexivity.
-          apply D_axiom; [prove_task_wf | apply /inP; reflexivity].
-        }
-        unfold safe_sub_f; simpl. apply D_axiom; [prove_task_wf | apply /inP; reflexivity].
-      - unfold replace_tm_f; simpl. apply D_axiom; [prove_task_wf | apply /inP; reflexivity].
+      wrewrite "Hz2".
+      wrewrite["Unit_def_r" (xt *r 0r)].
+      wreflexivity.
+      (*Alt (faster:)*)
+      (*wspecialize "Unit_def_r" (xt *r 0r).
+      wsymmetry.
+      wassumption.*)
     }
-    (*5. we can distribute and rewrite so that x * 0 + x * 0 = 0 + x * 0*)
-    apply (D_assert _ _ (Feq t_ty ((xt *r 0r) +r (xt *r 0r)) 
-      (0r +r (xt *r 0r)))).
+    (*Alt:*)
+    (* wrewrite["Mul_distr_l" xt 0r 0r]in "Hz3".*)
+    wspecialize "Mul_distr_l" xt 0r 0r.
+    wrewrite "Mul_distr_l" in "Hz3".
+    (*Now we use cancellation*)
+    wspecialize "add_cancel_l" (xt *r 0r) (xt *r 0r) 0r.
+    wapply "add_cancel_l".
+    wassumption.
+    (*Yay!*)
+  - (*Now we want to prove cancellation*)
+    wstart.
+    wintros "x" "y" "z" "Heq".
+    wassert "Hsub" (Feq t_ty ((-r xt) +r (xt +r yt)) ((-r xt) +r (xt +r zt))).
     {
-      (*need to rewrite, use symmetry, etc*)
-      admit.
+      wf_equal. wreflexivity. wassumption.
     }
-    (*Now, use cancellation*)
-    (*TODO: finish this (or make nicer with hypotheses)
-    This really isn't usable
-    what I should do 
-    1. name the hypotheses
-    2. make "derived derivations" - from core
-      that allow us to modify the hypotheses
-      (ex: specialize: 
-        if we have H: forall x, f in delta, 
-        then we can replace with H (f[t/x]))
-    3. On top of this, write tactics that
-      handle the reflexivity goals
-    *)
-    Check D_forallE.
-    apply (D_assert _ _ (safe_sub_f ))
-
-    (*4: we also have that x * 0 = 0 + x * 0*)
-    apply 
-
-
-        reflexivity.
+    (*rewrite with associativity*)
+    wrewrite<-["Assoc" (-r xt) xt yt]in "Hsub".
+    wrewrite<-["Assoc" (-r xt) xt zt]in "Hsub".
+    wrewrite["Inv_def_l" xt]in "Hsub".
+    wrewrite["Unit_def_l" yt]in "Hsub".
+    wrewrite["Unit_def_l" zt]in "Hsub".
+    wassumption.
+  - (*And an even easier goal*)
+    wstart.
+    wintros "x" "y" "Hxy".
+    (*TODO: tactic for this (easy with f_equal)*)
+    wassert "Heq" (Feq t_ty ((xt +r (-r yt)) +r yt) (0r +r yt)).
+    {
+      wf_equal. wassumption. wreflexivity.
     }
+    wrewrite["Assoc" xt (-r yt) yt]in "Heq".
+    wrewrite["Inv_def_l" yt]in "Heq".
+    wrewrite["Unit_def_r" xt]in "Heq".
+    wrewrite["Unit_def_l" yt]in "Heq".
+    wassumption.
+Qed.
 
-        admit.
+End RingTheory.
 
-        Search check_closed_tm.
-        
-        apply check_ty.
-      }
-      Check D_forallE.
-      apply D_forallE.
-
-      (Fquant Tforall x (Feq t_ty 
-      (Tfun op nil [Tfun unit nil nil; Tvar x]) (Tvar x)))
-
-
-      unfold Ring.ring. simpl.
-      assert (D_assert _ _ ())
-    }
-
-    apply /all_forallP.
-    2: prove_closed.
-
-
-
-    2: check_closed.
-    Search Logic.closed.
-    (*We want to prove that x * 0 = 0*)
-    (*First step: show that 0 + 0 = 0*)
-    apply D_assert (Feq t_ty (Tfun Ring.plus nil 
-      [Tfun Ring.zero nil nil; Tfun Ring.))
-    Check D_assert.
-    apply D_assert.
-
-
-
-    simpl.
-    unfold task_valid. simpl. split.
-    + prove_task_wf.
-    + intros.
-      unfold log_conseq. intros. simpl in H.
-      assert (L2 := H).
-      assert (L1 := H).
-      specialize (L1 _ (ltac:(left; reflexivity))).
-      specialize (L2 _ (ltac:(right; left; reflexivity))).
-      rewrite !tforall_rewrite. simpl.
-      intros.
-      (*TODO: how to avoid needing to unfold*) 
-      unfold safe_sub_f; simpl.
-      (*Let's see*)
-      (*assert: (x * (0+0) = x * 0)*)
-      assert (satisfies (task_gamma_valid w_wf) pd pf pf_full
-        (Feq t_ty (Tfun Ring.mult nil [Tvar (y0, t_ty); 
-          Tfun Ring.plus nil [Tfun Ring.zero nil nil; Tfun Ring.zero nil nil]])
-          (Tfun Ring.mult nil [Tvar x; Tfun Ring.zero nil nil])) ltac:(prove_fmla_ty)).
-      {
-        admit.
-      }
-      
-
-
-      }  Ring.zero nil nil])))
-      
-      simpl in *.
-
-      
-      simpl.
-      
-      simpl in L2.
-
-      
-      specialize (H0 _ ltac:(right; right)).
-    
-    
-    apply /check_task_wf_correct.
-
-      unfold check_task_wf.  
-      assert (check_context (theory_ctx_ext Ring.ring ++ [::])%list).
-        reflexivity.
-      rewrite H.
-      do 5 (try (apply /andP; split)); auto.
-      unfold task_delta.
-      rewrite all_cons.
-      apply /andP. split; auto.
-      rewrite all_cons. apply /andP. split; try reflexivity.
-      (*This is the hard one - one that doesnt work*)
-      rewrite theory_axioms_ext_equation_1.
-      rewrite !app_nil_r.
-      (*This should follow from above?*)
-      unfold Ring.ring.
-      unfold rev, catrev.
-      rewrite theory_axioms_ext_equation_4.
-      rewrite theory_axioms_ext_equation_4.
-      rewrite theory_axioms_ext_equation_8.
-      rewrite theory_axioms_ext_equation_8.
-      rewrite theory_axioms_ext_equation_2.
-      rewrite theory_axioms_ext_equation_2.
-      rewrite theory_axioms_ext_equation_2.
-      rewrite theory_axioms_ext_equation_2.
-      rewrite theory_axioms_ext_equation_2.
-      rewrite theory_axioms_ext_equation_1.
-      reflexivity.
-      unfold Assoc.assoc.
-      rewrite app_nil_r.
-      rewrite all_cons. unfold is_true. rewrite andb_true_iff. split; try reflexivity.
-
-      * reflexivity.
-      *
-      
-      apply /andP.
-      idtac.
-      reflexivity.
-      
-
-
-      rewrite !all_cons.
-      unfold is_true.
-      Search all cons.
-      simpl all.
-      cbn iota.
-      rewrite andb_true_iff.
-      apply /andP; split.
-      * reflexivity.
-      * unfold Ring.ring. unfold rev. unfold catrev.
-        rewrite theory_axioms_ext_equation_4.
-        cbn beta. unfold is_true. rewrite andb_true_iff.
-        split; try reflexivity.
-        unfold is_true.
-        cbn.
-
-        rewrite andb_true_iff. split; try reflexivity.
-
-      
-      
-      simpl catrev. simpl rev.
-      
-      
-      simpl. unfold theory_ctx_ext. apply /andP. split; try reflexivity.
-
-
-        simpl.
-        repeat (apply /andP; split; try reflexivity). idtac.
-        unfold sub_tys. unfold sub_from_map. simpl.
-
-        unfold get_exported_names.
-
-
-        reflexivity.
-        
-        reflexivity.
-      
-      unfold Ring.ring. simpl. reflexivity. apply /andP. split; try reflexivity.
-        simpl. rewrite -/all. simpl. rewrite -andbA. simpl. apply /andP. 
-
-
-      simpl.
-      simpl all.
-      simpl.
-      reflexivity.
-      compute.
-      simpl.
-
-
-      apply /andP. split.
-      rewrite <- !andbA.
-      do 3 (try (apply /andP; split)).
-      * auto.
-      * reflexivity.
-      * reflexivity.
-      repeat (apply /andP; split).
-      simpl.
-    
-    simpl.
-    reflexivity.
-    
-    prove_task_wf. *)
-
-(*Plan: prove cancellation, zero identity in ring*)
-
-(*THEN, do unit ring*)
-
-(*then prove 1 results about mult and -1*)
-
-(*Now, as a quick test, we prove some theorems about rings*)
-
-
-(*TODO: groups, comm groups, rings
-  Then, prove some ring theorems*)
-
-(*old, maybe get rid of after finishing ring theory*)
-(*Here, a simple test for cloning with a name and
-  substitution - fixed some bugs in Theory with this*)
-  (*Much simpler test*)
-  Module Test.
-
-  Definition theory1 : theory :=
-    rev [
-      tdef (abs_type t);
-      tdef (abs_fun op)
-    ].
-  (*Unlike why3, we require qualified names even in clone declaration*)
-  Definition tt : typesym := mk_ts "T.t" nil.
-  Definition tt_ty : vty := vty_cons tt nil.
-  Definition top : funsym := Build_funsym (Build_fpsym "T.op" nil [tt_ty; tt_ty] erefl erefl)
-    tt_ty erefl.
-  
-  Definition theory2 : theory :=
-    rev [
-      tdef (abs_type t);
-      tdef (abs_fun op);
-      tclone theory1 (Some "T"%string) [(tt, t)] [(top, op)] nil;
-      tprop Paxiom "foo" (fforalls [x; y] (Feq t_ty
-        (Tfun op nil [Tvar x; Tvar y])
-        (Tfun op nil [Tvar y; Tvar x])
-      ))
-    ].
-  
-  Lemma theory2_ctx: theory_ctx_int theory2 =
-    rev [abs_type t; abs_fun op].
-  Proof. reflexivity. Qed.
-  
-  Lemma theory2_ctx_ext: theory_ctx_ext theory2 =
-  rev [abs_type t; abs_fun op].
-  Proof.
-    reflexivity.
-  Qed.
-  
-  (*Typed*)
-  Lemma theory2_typed: typed_theory theory2.
-  Proof.
-    check_theory.
-  Qed.
-  
-  (*Well-formed*)
-  Lemma theory2_valid: valid_theory theory2.
-  Proof.
-    simpl. split; auto. prove_task_wf.
-  Qed.
-
-
-(*Test where we clone twice*)
-
-
-(*TODO: start here*)
-(*Want to see why we have issues in ring
-  I think - has to do with same module being cloned twice
-  Try: module with axiom, clone twice with different ops and names
-  then try with 1 that is unqualified
-  see if we find an issue
-  *)
-
-  Definition theory3 : theory :=
-    rev [
-      tdef (abs_type t);
-      tdef (abs_fun op);
-      tprop Paxiom "foo" (fforalls [x; y] (Feq t_ty
-        (Tfun op nil [Tvar x; Tvar y])
-        (Tfun op nil [Tvar y; Tvar x])
-      ))
-    ].
-
-    Definition at' : typesym := mk_ts "A.t" nil.
-    Definition at_ty' : vty := vty_cons at' nil.
-    Definition aop : funsym := Build_funsym (Build_fpsym "A.op" nil [at_ty'; at_ty'] erefl erefl)
-      at_ty' erefl.
-
-  Definition theory4 : theory :=
-    rev [
-      tdef (abs_type t);
-      tdef (abs_fun Ring.plus);
-      tdef (abs_fun Ring.mult);
-      tclone theory3 (Some "T"%string) [(tt, t)] [(top, Ring.plus)] nil;
-      tclone theory3 (Some "A"%string) [(at', t)] [(aop, Ring.mult)] nil;
-      tprop Paxiom "Mul_distr_l" (fforalls [x; y; z] (Feq t_ty
-        (Tfun Ring.mult nil [Tvar x; Tfun Ring.plus nil [Tvar y; Tvar z]])
-        (Tfun Ring.plus nil [Tfun Ring.mult nil [Tvar x; Tvar y]; Tfun Ring.mult nil [Tvar x; Tvar z]])
-      ))
-    ].
-
-  Lemma theory4_ctx: theory_ctx_int theory4 =
-    rev [abs_type t; abs_fun Ring.plus; abs_fun Ring.mult].
-  Proof. reflexivity. Qed.
-  
-  (*Typed*)
-  Lemma theory4_typed: typed_theory theory4.
-  Proof.
-    check_theory.
-  Qed.
-  
-  (*Well-formed*)
-  Lemma theory4_valid: valid_theory theory4.
-  Proof.
-    simpl. split; auto.
-    apply /check_task_wf_correct.
-    reflexivity.
-  Qed.
-    unfold check_task_wf.
-    apply /andP; split; auto.
-    apply /andP; split; auto.
-    apply /andP; split; auto.
-    apply /andP; split; auto.
-    apply /andP; split; auto.
-    2: {
-      simpl.
-      unfold theory3, rev, catrev.
-      rewrite !get_exported_names_equation_3.
-      rewrite !get_exported_names_equation_2.
-      rewrite !get_exported_names_equation_1.
-      rewrite !qualify_theory_equation_3.
-      rewrite !qualify_theory_equation_2.
-      rewrite !qualify_theory_equation_1.
-      simpl.
-      rewrite !theory_axioms_ext_equation_4.
-      rewrite !theory_axioms_ext_equation_2.
-      rewrite !theory_axioms_ext_equation_1.
-      unfold sub_props_map. Print sub_in_f.
-
-      simpl.
-      simpl.
-
-
-    } simpl.
-    
-    
-    2: reflexivity.
-    + simpl task_delta.
-      rewrite all_cons. apply /andP. split; auto.
-      unfold Assoc.assoc, rev, catrev.
-      rewrite !get_exported_names_equation_3.
-      rewrite !get_exported_names_equation_2.
-      rewrite get_exported_names_equation_1.
-      rewrite qualify_theory_equation_3.
-      rewrite !qualify_theory_equation_2.
-      rewrite qualify_theory_equation_1.
-      simpl.
-      rewrite theory_axioms_ext_equation_4.
-      rewrite !theory_axioms_ext_equation_2.
-      rewrite theory_axioms_ext_equation_1.
-      unfold sub_props_map. simpl List.map.
-      simpl map.
-      rewrite all_cons.
-      apply /andP; split; auto.
-      (*Aha, so this one is the problem*)
-      apply /typecheck_formula_correct.
-      apply F_Quant; auto.
-      {
-        apply /typecheck_type_correct. reflexivity.
-      }
-      simpl. apply F_Quant; auto.
-      {
-        apply /typecheck_type_correct. reflexivity.
-      }
-      simpl. apply F_Quant; auto.
-      {
-        apply /typecheck_type_correct. reflexivity.
-      }
-      apply F_Eq.
-      {
-        (*A problem here - why is everything op?*)
-        apply T_Fun; simpl; auto.
-        - apply /inP. reflexivity.
-        - apply /typecheck_type_correct. reflexivity.
-        -
-        
-        
-        repeat constructor; auto. apply /forallb_ForallP. reflexivity. unfold CommGroup.comm_group, Group.group, Comm.comm, Monoid.monoid, Assoc.assoc,
-        rev, catrev. 
-          simpl. rewrite !theory_ctx_ext_equation_3.
-          rewrite !theory_ctx_ext_equation_2.
-          rewrite theory_ctx_ext_equation_1.
-          simpl.
-          rewrite !theory_ctx_ext_equation_6.
-          simpl.
-          rewrite theory_ctx_ext_equation_1.
-          simpl.
-          rewrite !theory_ctx_ext_equation_3.
-          rewrite !theory_ctx_ext_equation_2.
-          rewrite !theory_ctx_ext_equation_6. simpl.
-          rewrite !theory_ctx_ext_equation_3.
-          rewrite !theory_ctx_ext_equation_2.
-          rewrite !theory_ctx_ext_equation_6. simpl.
-          rewrite !theory_ctx_ext_equation_3.
-          rewrite !theory_ctx_ext_equation_2.
-          rewrite !theory_ctx_ext_equation_1.
-          rewrite !app_nil_r.
-
-          simpl sig_f. unfold sig_f. simpl List.map.
-          unfold sub_funs.
-          unfold sub_from_map.
-          simpl get_assoc_list. simpl. auto.
-          (*WTF, this is true. What is going on?*)
-          simpl sub_funs.
-          unfold sub_funs. simpl.
-          unfold sub_ctx_map. simpl.
-          unfold Group.grou
-          simpl.
-          unfold sub_ctx_map.
-
-
-    simpl.
-    simpl.
-    Print Ltac prove_task_wf.
-    
-    prove_task_wf.
-  Qed.
-
-  Definition theory5 : theory :=
-    rev [
-      tdef (abs_type t);
-      tdef (abs_fun Ring.plus);
-      tdef (abs_fun Ring.mult);
-      tclone theory3 (Some "T"%string) [(tt, t)] [(top, Ring.plus)] nil;
-      tclone theory3 None [(t, t)] [(op, Ring.mult)] nil;
-      tprop Paxiom "Mul_distr_l" (fforalls [x; y; z] (Feq t_ty
-        (Tfun Ring.mult nil [Tvar x; Tfun Ring.plus nil [Tvar y; Tvar z]])
-        (Tfun Ring.plus nil [Tfun Ring.mult nil [Tvar x; Tvar y]; Tfun Ring.mult nil [Tvar x; Tvar z]])
-      ))
-    ].
-
-  Lemma theory5_ctx: theory_ctx_int theory5 =
-    rev [abs_type t; abs_fun Ring.plus; abs_fun Ring.mult].
-  Proof. reflexivity. Qed.
-  
-  (*Typed*)
-  Lemma theory4_typed: typed_theory theory4.
-  Proof.
-    check_theory.
-  Qed.
-  
-  (*Well-formed*)
-  Lemma theory4_valid: valid_theory theory2.
-  Proof.
-    simpl. split; auto. prove_task_wf.
-  Qed.
-
-      
-      
-    ].
-  
-  End Test.
+End Alg.
